prove return_unreachable_typing, do base case of lfilled_typing_skip

theories/interpreter_func.v
@@ -67,11 +67,10 @@ Inductive res_step : Type :=
 | RS_return : list value -> res_step
 | RS_normal : list administrative_instruction -> res_step.
 
-(* XXX unused? *)
-Fixpoint lholed_empty_vs lh : bool :=
+Fixpoint empty_base lh : bool :=
   match lh with
-  | LH_base [::] _ => true
-  | LH_rec [::] _ _ lh _ => lholed_empty_vs lh
+  | LH_base [::] [::] => true
+  | LH_rec _ _ _ lh _ => empty_base lh
   | _ => false
   end.
 
@@ -2504,6 +2503,69 @@ Proof.
   by apply/lfilledP.
 Qed.
 
+Lemma return_unreachable_typing : forall s C rvs es' t1s t2s,
+  e_typing s C (v_to_e_list rvs ++ [:: AI_basic BI_return] ++ es') (Tf t1s t2s) ->
+  e_typing s C (v_to_e_list rvs ++ [:: AI_basic BI_return]) (Tf t1s t2s).
+Proof.
+  intros s C rvs es' t1s t2s Hetype.
+  apply e_composition_typing in Hetype
+    as [ts [t1s' [t2s' [t3s [Ht1s [Ht2s [Hetypervs Hetype]]]]]]].
+  apply e_composition_typing in Hetype
+    as [ts' [t3s' [t2s'' [t4s' [Ht3s [Ht2s' [Hetyperet Hetypees']]]]]]].
+
+  subst t1s t2s.
+  apply et_composition' with (t2s := ts ++ t3s); apply ety_weakening => //.
+
+  apply et_to_bet in Hetyperet; last by auto_basic.
+  apply (Return_typing host_instance) in Hetyperet as [ts'' [ts''' [Ht3s' HretC]]].
+
+  apply ety_a'; first by auto_basic. subst.
+  apply bet_weakening.
+  by apply bet_return.
+Qed.
+
+Lemma lfilled_typing_skip: forall i lh s C e1s e2s es' t1s t2s rvs,
+  e_typing s C e1s (Tf t1s t2s) ->
+  empty_base lh ->
+  i > 0 ->
+  lfilledInd i lh (v_to_e_list rvs ++ [:: AI_basic BI_return] ++ es') e1s ->
+  lfilledInd i lh (v_to_e_list rvs ++ [:: AI_basic BI_return]) e2s ->
+  e_typing s C e2s (Tf t1s t2s).
+Proof.
+  induction i as [|i] => //;
+    intros lh s C e1s e2s es' t1s t2s rvs Hetype Hbase Hi Hlf1 Hlf2.
+  destruct i => //.
+  - inversion Hlf1 as [|??? les lh' ???? Hlf1'].
+    inversion Hlf2 as [|????????? Hlf2' Heqk Heqlh].
+    (* deduce that lh' is used for both Hlf1' and Hlf2' *)
+    subst. inversion Heqlh; clear Heqlh. subst.
+    (* deduce that lh' is a base *)
+    destruct lh' as [lh_vs lh_es|]; try by inversion Hlf1'.
+    (* use empty_base lh' *)
+    destruct lh_vs, lh_es => //.
+    inversion Hlf1'; inversion Hlf2'; simpl in *; subst.
+    clear Hlf1 Hlf2 Hlf1' Hlf2' IHi Hi.
+    rewrite cats0 -cat1s in Hetype.
+
+    apply e_composition_typing in Hetype
+      as [ts [t1s' [t2s' [t3s [Ht1s [Ht2s [Hetypervs Hetype]]]]]]].
+    apply e_composition_typing in Hetype
+      as [ts' [t3s' [t2s'' [t4s' [Ht3s [Ht2s' [Hetypelab Hetypees'']]]]]]].
+
+    rewrite cats0 -cat1s. subst t1s t2s.
+    apply et_composition' with (t2s := ts ++ t3s); apply ety_weakening => //.
+    subst t2s' t3s.
+    apply et_composition' with (t2s := ts' ++ t4s'); apply ety_weakening => //.
+
+    apply Label_typing in Hetypelab
+      as [label_ts [t3s'' [Heqt4s' [Hetypeles [HetypeLI Hlen]]]]].
+
+    subst t4s'; apply et_weakening_empty_1.
+    apply ety_label with (ts := label_ts) => //.
+    by apply return_unreachable_typing in HetypeLI.
+
+Admitted.
+
 (* XXX none of the existing lemmas Lfilled_return_typing etc
  * give us this result because they don't have the empty_vs_base assumption,
  * which is necessary to assert that rvs are all the values we need to consider *)
@@ -2569,7 +2631,6 @@ Proof.
     apply e_composition_typing in Hetype
       as [ts'' [t0s [t3s [t2s' [Ht0s [Hts' [Hetypelab Hetype]]]]]]].
 
-    Check Label_typing.
     apply Label_typing in Hetypelab
       as [label_ts [t2s'' [Heqt2s' [Hetypees' [HetypeLI Hlen]]]]].
 
